Runtime/Network/Execution/ReactionOutput.lean
@@ -2,46 +2,38 @@ import Runtime.Network.Execution.Basic
 
 namespace Network.Executable
 
+open Graph.Class
+
 structure ReactionOutput (exec : Executable net) where
   reactor : ReactorId net
-  reaction : reactor.class.reactionType
-  raw : reaction.outputType exec.tag.time
+  reaction : ReactionType reactor.class
+  raw : reaction.val.outputType exec.tag.time
 
 namespace ReactionOutput
 
 variable {exec : Executable net}
 
-def fromRaw {reactor : ReactorId net} {reaction : reactor.class.reactionType} (raw : reaction.outputType exec.tag.time) : ReactionOutput exec :=
+def fromRaw {reactor : ReactorId net} {reaction : ReactionType reactor.class} (raw : reaction.val.outputType exec.tag.time) : ReactionOutput exec :=
   { reactor, reaction, raw }
 
 def events (output : ReactionOutput exec) :=
-  output.raw.events.map fun event => Event.action event.time ⟨output.reactor, event.action⟩ event.value
-
--- Note: This theorem is really only needed for `ReactionOutput.local`.
-private def local_type_correctness {output : ReactionOutput exec} {port port'} : 
-  (output.reaction.portEffectsInjCoe.inv (.inl port) = some port') → 
-  (output.reactor.class.reactionOutputScheme |>.restrict output.reaction.portEffects |>.type port') = 
-  output.reactor.outputs.type port :=
-  (by rw [Interface.Scheme.restrict_type, output.reaction.portEffectsInjCoe.invCoeId _ ·])
+  output.raw.events.map fun event => 
+    Event.action 
+      event.time 
+      ⟨output.reactor, output.reaction.subAE.coe event.action⟩ 
+      (output.reaction.subAE.coeEqType ▸ event.value)
 
 def «local» (output : ReactionOutput exec) (port : output.reactor.outputs.vars) : Option (output.reactor.outputs.type port) := 
-  match h : output.reaction.portEffectsInjCoe.inv (.inl port) with
+  match h : output.reaction.subPE.inv (.inl port) with
   | none => none -- independent port
-  | some port' => local_type_correctness h ▸ output.raw.ports port'
-
--- Note: This theorem is really only needed for `ReactionOutput.child'`.
-private def child'_type_correctness {output : ReactionOutput exec} {child : ReactorId.Child output.reactor} {port port'} : 
-  (output.reaction.portEffectsInjCoe.inv (.inr ⟨child.class, port⟩) = some port') →
-  ((output.reactor.class.reactionOutputScheme).restrict output.reaction.portEffects).type port' =
-  (child.class.class.interface .inputs).type port :=
-  (by rw [Interface.Scheme.restrict_type, output.reaction.portEffectsInjCoe.invCoeId _ ·]; rfl)
+  | some port' => output.reaction.subPE.invEqType h ▸ output.raw.ports port'
 
 -- This function implements the core of the `child` function below.
 -- It's only missing some type casts for the `port` (and consequently the return type).
 private def child' (output : ReactionOutput exec) {child : ReactorId.Child output.reactor} (port : (child.class.class.interface .inputs).vars) : Option (child.class.class.interface .inputs |>.type port) := 
-  match h : output.reaction.portEffectsInjCoe.inv (.inr ⟨child.class, port⟩) with
+  match h : output.reaction.subPE.inv (.inr ⟨child.class, port⟩) with
   | none => none -- independent port
-  | some port' => child'_type_correctness h ▸ output.raw.ports port'
+  | some port' => output.reaction.subPE.invEqType h ▸ output.raw.ports port'
 
 private theorem child_type_correctness {reactor : ReactorId net} {child : ReactorId.Child reactor} {port} :
   (child.class.class.interface .inputs).type (Graph.Path.Child.class_eq_class ▸ port) = (child.val.inputs).type port := by
