Runtime/Network/Graph/Path/Basic.lean
@@ -50,17 +50,5 @@ theorem cons_class : (Path.cons child subpath).class = subpath.class := rfl
 @[simp]
 theorem eq_class_iff_cons_eq_class : (path₁.class = path₂.class) ↔ (Path.cons child₁ path₁).class = (Path.cons child₂ path₂).class := ⟨id, id⟩
 
-instance {path : Path graph start} {reaction : path.class.reactionType} : 
-  InjectiveCoe reaction.portSources path.class.reactionInputScheme.vars :=
-  reaction.portSourcesInjCoe
-
-instance {path : Path graph start} {reaction : path.class.reactionType} : 
-  InjectiveCoe reaction.portEffects path.class.reactionOutputScheme.vars :=
-  reaction.portEffectsInjCoe
-
-instance {path : Path graph start} {reaction : path.class.reactionType} : 
-  InjectiveCoe reaction.actionSources (path.class.interface .actions).vars :=
-  reaction.actionSourcesInjCoe
-
 end Path
 end Network.Graph
