Runtime/Utilities/Extensions.lean
@@ -1,15 +1,5 @@
 import Runtime.Time
 
-macro "invInjProof" : tactic => `(tactic| first | (intro _ _ _ h₁ h₂; simp at h₁ h₂; split at h₁ <;> split at h₂ <;> first | rfl | contradiction | simp [←h₁] at h₂) | simp)
-macro "coeInvIdProof" : tactic => `(tactic| try (intro a; cases a <;> rfl))
-class InjectiveCoe (α β) extends Coe α β where
-  inv      : β → Option α
-  invInj   : ∀ {b₁ b₂ a}, (inv b₁ = some a) → (inv b₂ = some a) → (b₁ = b₂) := by invInjProof
-  coeInvId : ∀ a, inv (coe a) = a := by coeInvIdProof
-  
-theorem InjectiveCoe.invCoeId [inst : InjectiveCoe α β] : ∀ b, (inst.inv b = some a) → (inst.coe a = b) := 
-  fun _ h => (invInj h <| inst.coeInvId a).symm  
-
 def Array.unique (as : Array α) (f : α → β) [DecidableEq β] : (Array α) × (Array α) := Id.run do
   let mut included : Array α := #[] 
   let mut excluded : Array α := #[]
